feat: more lemmas about counting and cardinality

Fifteen/Logic/BishodFin.lean
@@ -3,6 +3,8 @@ Copyright (c) 2023 Jun Yoshida. All rights reserved.
 Released under Apache 2.0 license as described in the file LICENSE.
 -/
 
+import Std.Tactic.Basic
+
 import Fifteen.Data.List.Basic
 
 /-!
@@ -36,7 +38,7 @@ section Basic
 
 /-! ### Basic declarations -/
 
-variable {α : Type u} [BishopFin α]
+variable {α : Type u} {β : Type v} [BishopFin α] [BishopFin β]
 
 variable (α) in
 /--
@@ -61,8 +63,41 @@ variable (α) in
 def card : Nat :=
   (elems α).length
 
-theorem _root_.List.Nodup.length_le_card [DecidableEq α] {l : List α} (nodup : l.Nodup) : l.length ≤ card α :=
+theorem _root_.List.Nodup.length_le_card {l : List α} (nodup : l.Nodup) : l.length ≤ card α :=
   nodup.length_le_of_subset <| subset_elems l
+
+theorem card_le_card_of_inj (f : α → β) (f_inj : ∀ a₁ a₂, f a₁ = f a₂ → a₁ = a₂) : card α ≤ card β := by
+  dsimp only [card]
+  conv =>
+    lhs; equals ((elems α).map f).length => rw [List.length_map]
+  refine List.Nodup.length_le_of_subset ?_ ?_
+  . exact nodup_elems.map f f_inj
+  . exact subset_elems _
+
+theorem card_ge_card_of_surj (f : α → β) (f_surj : ∀ b, ∃ a, f a = b) : card α ≥ card β := by
+  dsimp only [card]
+  conv =>
+    lhs; equals ((elems α).map f).length => rw [List.length_map]
+  refine nodup_elems.length_le_of_subset ?_
+  intro b _
+  simp only [List.mem_map, mem_elems, true_and]
+  exact f_surj b
+
+theorem card_eq_card_of_bij [BishopFin β] (f : α → β) (f_surj : ∀ b, ∃ a, f a = b) (f_inj : ∀ a₁ a₂, f a₁ = f a₂ → a₁ = a₂) : card α = card β := by
+  refine Nat.le_antisymm ?_ ?_
+  . exact card_le_card_of_inj f f_inj
+  . exact card_ge_card_of_surj f f_surj
+
+theorem card_eq_card_of_inv (f : α → β) (g : β → α) (hgf : ∀ a, g (f a) = a) (hfg : ∀ b, f (g b) = b) : card α = card β := by
+  refine Nat.le_antisymm ?_ ?_
+  . show card α ≤ card β
+    refine card_le_card_of_inj f ?_
+    intros a₁ a₂ hfa
+    rw [← hgf a₁, ← hgf a₂, hfa]
+  . show card β ≤ card α
+    refine card_le_card_of_inj g ?_
+    intro b₁ b₂ hgb
+    rw [← hfg b₁, ← hfg b₂, hgb]
 
 instance (priority:=0) decidableEx (p : α → Prop) [DecidablePred p] : Decidable (∃ a, p a) :=
   if hp : ∃ a, (a ∈ elems α ∧ p a) then
@@ -112,24 +147,37 @@ instance subtype {α : Type u} {p : α → Prop} [BishopFin α] [DecidablePred p
     simp only [List.mem_pmap, List.mem_filter, mem_elems, true_and, decide_eq_true_eq]
     exact ⟨a.1, a.2, a.2, rfl⟩
 
+theorem card_subset_le_card {α : Type u} {p : α → Prop} [BishopFin α] [DecidablePred p] : card {a // p a} ≤ card α := by
+  apply card_le_card_of_inj Subtype.val
+  intro _ _; exact Subtype.eq
+
 
 /-! ### Counting elements -/
 
 section Count
 
-variable {α : Type u} [BishopFin α]
+variable {α : Type u} {β : Type v} [BishopFin α] [BishopFin β]
 
 /-- Counting the number of elements in a Bishop finite type `α` satisfying a decidable predicate `p : α → Prop`. -/
 @[inline]
 def count (p : α → Prop) [DecidablePred p] : Nat :=
-  BishopFin.elems α |>.countP fun i => decide (p i)
+  BishopFin.elems α |>.countP fun a => decide (p a)
 
-theorem count_eq_card {p : α → Prop} [DecidablePred p] : count p = card {a // p a} := by
+@[inherit_doc BishopFin.count] syntax "#| " withoutPosition(ident (" : " term)? " // " term) " |" : term
+
+scoped macro_rules
+| `(#| $x : $type // $p |) => ``(BishopFin.count (fun ($x:ident : $type) => $p))
+| `(#| $x // $p |)         => ``(BishopFin.count (fun ($x:ident : _) => $p))
+
+
+variable {p q : α → Prop} [DecidablePred p] [DecidablePred q]
+
+theorem count_eq_card : count p = card {a // p a} := by
   dsimp [count]; rewrite [List.countP_eq_length_filter]
   conv => rhs; change subtype (p:=p) |>.elems' |>.length
   dsimp [elems']; simp only [List.length_pmap]
 
-theorem count_le {p : α → Prop} [DecidablePred p] : count p ≤ card α :=
+theorem count_le : count p ≤ card α :=
   List.countP_le_length _
 
 @[simp]
@@ -140,22 +188,110 @@ theorem count_true : count (fun (_ : α) => True) = card α := by
 theorem count_false : count (fun (_ : α) => False) = 0 :=
   List.countP_false
 
-theorem count_mono_left {p q : α → Prop} [DecidablePred p] [DecidablePred q] (h : ∀ a, p a → q a) : count p ≤ count q :=
+theorem count_mono_left (h : ∀ a, p a → q a) : count p ≤ count q :=
   List.countP_mono_left fun a _ ha =>
     have : q a := h a (of_decide_eq_true ha)
     decide_eq_true this
 
+theorem count_congr (h : ∀ a, p a ↔ q a) : count p = count q :=
+  Nat.le_antisymm
+    (count_mono_left fun a => (h a).1)
+    (count_mono_left fun a => (h a).2)
+
+theorem count_eq_count_sub (h : ∀ a, p a → q a) : count p = count (p ∘ Subtype.val (p:=q)) := by
+  iterate rewrite [count_eq_card]
+  refine card_eq_card_of_inv ?f ?g ?hgf ?hfg
+  . exact fun x => ⟨⟨x.1, h x.1 x.2⟩, x.2⟩
+  . exact fun y => ⟨y.1.1, y.2⟩
+  all_goals simp
+
 @[simp]
-theorem count_le_one_of_unique (p : α → Prop) [DecidablePred p] (p_unique : ∀ a b, p a → p b → a = b) : count p ≤ 1 := by
+theorem count_le_one_of_unique (p_unique : ∀ a b, p a → p b → a = b) : count p ≤ 1 := by
   dsimp [count]
   refine List.countP_le_one_of_unique_nodup ?_ nodup_elems
   simp only [decide_eq_true_eq]
   exact p_unique
 
-theorem count_image_le {β : Type v} [DecidableEq β] [BishopFin β] (f : α → β) : count (fun b => ∃ a, f a = b) ≤ card α := by
+variable (p) in
+theorem card_eq_count_add_count_not : card α = count p + count (fun a => ¬ p a) := by
+  dsimp [card]
+  rewrite [(elems α).length_eq_countP_add_countP p]
+  apply congrArg (count p + ·)
+  simp only [decide_eq_true_eq]
+  rfl
+
+theorem count_or_le_add : count (fun a => p a ∨ q a) ≤ count p + count q := by
+  dsimp [count]; simp only [decide_or, List.countP_or_le_add]
+
+theorem count_disjoint_or (h : ∀ a, ¬(p a ∧ q a)) : count (fun a => p a ∨ q a) = count p + count q := by
+  dsimp [count]; simp only [decide_or]
+  apply List.countP_disjoint
+  simp only [← decide_and, decide_eq_false_iff_not]
+  exact h
+
+theorem count_image_le_card [DecidableEq β] (f : α → β) : count (fun b => ∃ a, f a = b) ≤ card α := by
   have := (elems α).countP_image_le_length nodup_elems (f := f)
   simp only [mem_elems, true_and] at this
   exact this
+
+theorem count_image_le_count [DecidableEq β] (f : α → β) : count (fun b => ∃ a, p a ∧ f a = b) ≤ count p := by
+  conv => rhs; rewrite [count_eq_card]
+  refine trans (r:=Eq) ?_ (count_image_le_card (f ∘ Subtype.val))
+  apply count_congr
+  intro b; constructor
+  . intro h; let ⟨a,hpa,hfa⟩ := h
+    exact ⟨⟨a,hpa⟩, hfa⟩
+  . intro h; let ⟨⟨a,hpa⟩,hfa⟩ := h
+    exact ⟨a,hpa,hfa⟩
+
+theorem count_le_count_invimage [DecidableEq α] (f : β → α) (hf : ∀ a, p a → ∃ b, f b = a) : count p ≤ count (p ∘ f) := by
+  rewrite [count_eq_count_sub hf]
+  let f' : β → {a // ∃ b, f b = a} := fun b => ⟨f b, b, rfl⟩
+  have : f = Subtype.val ∘ f' := funext fun _ => rfl
+  rewrite [this]
+  dsimp [count]
+  conv =>
+    rhs; equals ((elems β).map f').countP (fun a => decide (p a.val)) =>
+      rewrite [List.countP_map]; rfl
+  refine List.countP_mono_right ?_ nodup_elems
+  intro x _; simp only [List.mem_map]
+  let ⟨a,b,ha⟩ := x
+  exists b; apply And.intro (mem_elems b)
+  exact Subtype.eq ha
+
+/--
+:::note info
+In contrast to `BishopFin.count_le_count_invimage`, this function does not require `DecidableEq α`.
+:::
+-/
+theorem count_le_count_invimage_of_surj (f : β → α) (f_surj : ∀ a, ∃ b, f b = a) : count p ≤ count (p ∘ f) := by
+  iterate rewrite [count_eq_card]
+  refine card_ge_card_of_surj ?f ?f_surj
+  . exact fun y => ⟨f y.1, y.2⟩
+  . intro x
+    let ⟨a,ha⟩ := x
+    let ⟨b,hb⟩ := f_surj a
+    exists ⟨b, by dsimp; exact hb ▸ ha⟩
+    exact Subtype.eq hb
+
+theorem count_invimage_le_count_of_inj (f : β → α) (f_inj : ∀ b₁ b₂, f b₁ = f b₂ → b₁ = b₂) : count (p ∘ f) ≤ count p := by
+  iterate rewrite [count_eq_card]
+  refine card_le_card_of_inj ?f ?f_inj
+  . exact fun y => ⟨f y.1, y.2⟩
+  . intro y₁ y₂ h
+    apply Subtype.eq; apply f_inj
+    exact congrArg Subtype.val h
+
+theorem count_eq_count_invimage_of_bij (f : β → α) (f_surj : ∀ a, ∃ b, f b = a)  (f_inj : ∀ b₁ b₂, f b₁ = f b₂ → b₁ = b₂) : count p = count (p ∘ f) := by
+  refine Nat.le_antisymm ?_ ?_
+  . exact count_le_count_invimage_of_surj f f_surj
+  . exact count_invimage_le_count_of_inj f f_inj
+
+theorem count_eq_count_invimage_of_inv (f : β → α) (g : α → β) (hgf : ∀ b, g (f b) = b) (hfg : ∀ a, f (g a) = a) : count p = count (p ∘ f) := by
+  refine count_eq_count_invimage_of_bij f ?_ ?_
+  . exact fun a => ⟨g a, hfg a⟩
+  . intro b₁ b₂ hb
+    rw [← hgf b₁, ← hgf b₂, hb]
 
 end Count
 
